theories/zoo_parabs/waiters__types.v
@@ -2,7 +2,7 @@ Require Import zoo.prelude.
 Require Import zoo.language.typeclasses.
 Require Import zoo.language.notations.
 Require Export zoo_parabs.waiter.
-Require Export zoo_saturn.mpmc_queue_1.
+Require Export zoo_saturn.queue_mpmc_1.
 Require Export zoo_std.array.
 Require Import zoo.options.
 
