theories/zoo_saturn/queue_mpmc_1__code.v
@@ -1,0 +1,115 @@
+Require Import zoo.prelude.
+Require Import zoo.language.typeclasses.
+Require Import zoo.language.notations.
+Require Import zoo_std.domain.
+Require Import zoo.options.
+
+Notation "'queue_mpmc_1٠Null'" := (
+  in_type "zoo_saturn.queue_mpmc_1.node" 0
+)(in custom zoo_tag
+).
+Notation "'queue_mpmc_1٠Node'" := (
+  in_type "zoo_saturn.queue_mpmc_1.node" 1
+)(in custom zoo_tag
+).
+
+Notation "'queue_mpmc_1٠next'" := (
+  in_type "zoo_saturn.queue_mpmc_1.node.Node" 0
+)(in custom zoo_field
+).
+Notation "'queue_mpmc_1٠data'" := (
+  in_type "zoo_saturn.queue_mpmc_1.node.Node" 1
+)(in custom zoo_field
+).
+
+Notation "'queue_mpmc_1٠front'" := (
+  in_type "zoo_saturn.queue_mpmc_1.t" 0
+)(in custom zoo_field
+).
+Notation "'queue_mpmc_1٠back'" := (
+  in_type "zoo_saturn.queue_mpmc_1.t" 1
+)(in custom zoo_field
+).
+
+Definition queue_mpmc_1٠create : val :=
+  𝗳𝘂𝗻 ⎽ ->
+    𝗹𝗲𝘁 "front" =
+      ‘queue_mpmc_1٠Node{ §queue_mpmc_1٠Null, () }
+    𝗶𝗻
+    { "front", "front" }.
+
+Definition queue_mpmc_1٠is_empty : val :=
+  𝗳𝘂𝗻 "t" ->
+    𝗺𝗮𝘁𝗰𝗵 "t".{queue_mpmc_1٠front} 𝘄𝗶𝘁𝗵
+    | queue_mpmc_1٠Node ⎽ ⎽ 𝗮𝘀 "front_r" ->
+        "front_r".{queue_mpmc_1٠next} == §queue_mpmc_1٠Null
+    𝗲𝗻𝗱.
+
+Definition queue_mpmc_1٠push₁ : val :=
+  𝗿𝗲𝗰 "push" "node" "new_back" ->
+    𝗺𝗮𝘁𝗰𝗵 "node" 𝘄𝗶𝘁𝗵
+    | queue_mpmc_1٠Node ⎽ ⎽ 𝗮𝘀 "node_r" ->
+        𝗺𝗮𝘁𝗰𝗵 "node_r".{queue_mpmc_1٠next} 𝘄𝗶𝘁𝗵
+        | queue_mpmc_1٠Node ⎽ ⎽ 𝗮𝘀 "next" ->
+            "push" "next" "new_back"
+        | queue_mpmc_1٠Null ->
+            𝗶𝗳
+              ~
+              𝗰𝗮𝘀
+                "node_r".[queue_mpmc_1٠next]
+                §queue_mpmc_1٠Null
+                "new_back"
+            𝘁𝗵𝗲𝗻 (
+              domain٠yield () ⍮
+              "push" "node" "new_back"
+            )
+        𝗲𝗻𝗱
+    𝗲𝗻𝗱.
+
+Definition queue_mpmc_1٠fix_back : val :=
+  𝗿𝗲𝗰 "fix_back" "t" "back" "new_back" ->
+    𝗺𝗮𝘁𝗰𝗵 "new_back" 𝘄𝗶𝘁𝗵
+    | queue_mpmc_1٠Node ⎽ ⎽ 𝗮𝘀 "new_back_r" ->
+        𝗶𝗳
+          "new_back_r".{queue_mpmc_1٠next} == §queue_mpmc_1٠Null
+          𝗮𝗻𝗱
+          ~ 𝗰𝗮𝘀 "t".[queue_mpmc_1٠back] "back" "new_back"
+        𝘁𝗵𝗲𝗻 (
+          domain٠yield () ⍮
+          "fix_back" "t" "t".{queue_mpmc_1٠back} "new_back"
+        )
+    𝗲𝗻𝗱.
+
+Definition queue_mpmc_1٠push : val :=
+  𝗳𝘂𝗻 "t" "v" ->
+    𝗺𝗮𝘁𝗰𝗵
+      ‘queue_mpmc_1٠Node{ §queue_mpmc_1٠Null, "v" }
+    𝘄𝗶𝘁𝗵
+    | queue_mpmc_1٠Node ⎽ ⎽ 𝗮𝘀 "new_back" ->
+        𝗹𝗲𝘁 "back" = "t".{queue_mpmc_1٠back} 𝗶𝗻
+        queue_mpmc_1٠push₁ "back" "new_back" ⍮
+        queue_mpmc_1٠fix_back "t" "back" "new_back"
+    𝗲𝗻𝗱.
+
+Definition queue_mpmc_1٠pop : val :=
+  𝗿𝗲𝗰 "pop" "t" ->
+    𝗺𝗮𝘁𝗰𝗵 "t".{queue_mpmc_1٠front} 𝘄𝗶𝘁𝗵
+    | queue_mpmc_1٠Node ⎽ ⎽ 𝗮𝘀 "front" ->
+        𝗹𝗲𝘁 "front_r" = "front" 𝗶𝗻
+        𝗺𝗮𝘁𝗰𝗵 "front_r".{queue_mpmc_1٠next} 𝘄𝗶𝘁𝗵
+        | queue_mpmc_1٠Null ->
+            §None
+        | queue_mpmc_1٠Node ⎽ ⎽ 𝗮𝘀 "new_front" ->
+            𝗹𝗲𝘁 "new_front_r" = "new_front" 𝗶𝗻
+            𝗶𝗳
+              𝗰𝗮𝘀 "t".[queue_mpmc_1٠front] "front" "new_front"
+            𝘁𝗵𝗲𝗻 (
+              𝗹𝗲𝘁 "v" = "new_front_r".{queue_mpmc_1٠data} 𝗶𝗻
+              "new_front_r" <-{queue_mpmc_1٠data} () ⍮
+              ‘Some( "v" )
+            ) 𝗲𝗹𝘀𝗲 (
+              domain٠yield () ⍮
+              "pop" "t"
+            )
+        𝗲𝗻𝗱
+    𝗲𝗻𝗱.
