theories/zoo_saturn/queue_mpmc_1__opaque.v
@@ -1,0 +1,8 @@
+Require Import zoo_saturn.queue_mpmc_1__code.
+
+#[global] Opaque queue_mpmc_1٠create.
+#[global] Opaque queue_mpmc_1٠is_empty.
+#[global] Opaque queue_mpmc_1٠push₁.
+#[global] Opaque queue_mpmc_1٠fix_back.
+#[global] Opaque queue_mpmc_1٠push.
+#[global] Opaque queue_mpmc_1٠pop.
